<rdf:RDF
    xmlns:vs="http://www.w3.org/2003/06/sw-vocab-status/ns#"
    xmlns:ldp="http://www.w3.org/ns/ldp#"
    xmlns:version="http://purl.org/linked-data/version#"
    xmlns:dct="http://purl.org/dc/terms/"
    xmlns:dc="http://purl.org/dc/elements/1.1/"
    xmlns:ui="http://purl.org/linked-data/registry-ui#"
    xmlns:prov="http://www.w3.org/ns/prov#"
    xmlns:skos="http://www.w3.org/2004/02/skos/core#"
    xmlns:qudt-dimension="http://qudt.org/vocab/dimension#"
    xmlns:ssd="http://www.w3.org/ns/sparql-service-description#"
    xmlns:vann="http://purl.org/vocab/vann/"
    xmlns:cc="http://creativecommons.org/ns#"
    xmlns:xsd="http://www.w3.org/2001/XMLSchema#"
    xmlns:rdf="http://www.w3.org/1999/02/22-rdf-syntax-ns#"
    xmlns:reg="http://purl.org/linked-data/registry#"
    xmlns:bufr4-core="http://codes.wmo.int/bufr4/schema/core/"
    xmlns:rdfs="http://www.w3.org/2000/01/rdf-schema#"
    xmlns:void="http://rdfs.org/ns/void#"
    xmlns:time="http://www.w3.org/2006/time#"
    xmlns:dgu="http://reference.data.gov.uk/def/reference/"
    xmlns:common-unit="http://codes.wmo.int/common/schema/unit/"
    xmlns:common-core="http://codes.wmo.int/common/schema/core/"
    xmlns:qudt="http://qudt.org/schema/qudt#"
    xmlns:owl="http://www.w3.org/2002/07/owl#"
    xmlns:qb="http://purl.org/linked-data/cube#"
    xmlns:grib2-parameter="http://codes.wmo.int/grib2/schema/parameter/"
    xmlns:qudt-unit="http://qudt.org/vocab/unit#"
    xmlns:qudt-quantity="http://qudt.org/vocab/quantity#"
    xmlns:api="http://purl.org/linked-data/api/vocab#"
    xmlns:foaf="http://xmlns.com/foaf/0.1/"
    xmlns:grib2-core="http://codes.wmo.int/grib2/schema/core/">
  <skos:Collection rdf:about="http://codes.wmo.int/wmdr/ReferenceSurfaceType">
    <skos:member>
      <skos:Concept rdf:about="http://codes.wmo.int/wmdr/ReferenceSurfaceType/seaSurface">
        <dct:description xml:lang="en">The natural surface of the sea at the interface between the atmosphere and the ocean</dct:description>
        <rdfs:label>sea surface</rdfs:label>
        <skos:notation>seaSurface</skos:notation>
      </skos:Concept>
    </skos:member>
    <owl:versionInfo rdf:datatype="http://www.w3.org/2001/XMLSchema#integer"
    >3</owl:versionInfo>
    <skos:member>
      <skos:Concept rdf:about="http://codes.wmo.int/wmdr/ReferenceSurfaceType/roofTerrace">
        <dct:description xml:lang="en">The roof or terrace of a building, elevated with respect to the surrounding local ground</dct:description>
        <rdfs:label>roof or terrace</rdfs:label>
        <skos:notation>roofTerrace</skos:notation>
      </skos:Concept>
    </skos:member>
    <skos:member>
      <skos:Concept rdf:about="http://codes.wmo.int/wmdr/ReferenceSurfaceType/deck">
        <dct:description xml:lang="en">A permanent covering over a compartment or the body of a fixed or mobile platform (ship). Also the horizontal structure that forms the roof of the hull, elevated with respect to the surrounding sea surface</dct:description>
        <rdfs:label>deck</rdfs:label>
        <skos:notation>deck</skos:notation>
      </skos:Concept>
    </skos:member>
    <skos:member>
      <skos:Concept rdf:about="http://codes.wmo.int/wmdr/ReferenceSurfaceType/unknown">
        <dct:description xml:lang="en">The reference surface is unknown</dct:description>
        <rdfs:label>unknown</rdfs:label>
        <skos:notation>unknown</skos:notation>
      </skos:Concept>
    </skos:member>
    <skos:member>
      <skos:Concept rdf:about="http://codes.wmo.int/wmdr/ReferenceSurfaceType/artificialGround">
        <dct:description xml:lang="en">An artificial surface at the interface between the atmosphere and the terrestrial globe, not elevated with respect to the nearby surrounding area (on a scale of 50 meters)</dct:description>
        <rdfs:label>artificial ground</rdfs:label>
        <skos:notation>artificialGround</skos:notation>
      </skos:Concept>
    </skos:member>
    <rdfs:label>Type of reference surface</rdfs:label>
    <ldp:hasMemberRelation rdf:resource="http://www.w3.org/2004/02/skos/core#member"/>
    <skos:member>
      <skos:Concept rdf:about="http://codes.wmo.int/wmdr/ReferenceSurfaceType/naturalGround">
        <dct:description xml:lang="en">The natural surface at the interface between the atmosphere and the terrestrial globe, not elevated with respect to the nearby surrounding area (on a scale of 50 meters)</dct:description>
        <rdfs:label>natural ground</rdfs:label>
        <skos:notation>naturalGround</skos:notation>
      </skos:Concept>
    </skos:member>
    <dct:modified rdf:datatype="http://www.w3.org/2001/XMLSchema#dateTime"
    >2019-11-21T09:23:47.456Z</dct:modified>
    <rdf:type rdf:resource="http://purl.org/linked-data/registry#Register"/>
    <dct:description>Type of reference surface</dct:description>
    <rdf:type rdf:resource="http://www.w3.org/ns/ldp#Container"/>
    <skos:member>
      <skos:Concept rdf:about="http://codes.wmo.int/wmdr/ReferenceSurfaceType/inapplicable">
        <dct:description xml:lang="en">None of the codes in the table are applicable in the context of the reference surface</dct:description>
        <rdfs:label>inapplicable</rdfs:label>
        <skos:notation>inapplicable</skos:notation>
      </skos:Concept>
    </skos:member>
  </skos:Collection>
</rdf:RDF>
